Faster mergesort implementation

MergeSort.v
@@ -19,7 +19,7 @@ Proof.
     end; eauto.
 Qed.
 
-Lemma Forall_rev_iff A (P : A -> Prop) xs :
+Corollary Forall_rev_iff A (P : A -> Prop) xs :
   Forall P (rev xs) <-> Forall P xs.
 Proof.
   split;
@@ -30,6 +30,25 @@ Proof.
     eapply Forall_forall in HForall;
     eauto.
 Qed.
+
+Definition Forall_rev_inv A P xs := proj1 (Forall_rev_iff A P xs).
+Definition Forall_rev A P xs := proj2 (Forall_rev_iff A P xs).
+
+Corollary Forall_map_iff A B P (f : A -> B) xs :
+  Forall P (map f xs) <-> Forall (fun x => P (f x)) xs.
+Proof.
+  split;
+    intros HForall;
+    apply Forall_forall;
+    intros ? HIn;
+    [ eapply in_map in HIn
+    | apply in_map_iff in HIn; destruct HIn as [? []]; subst ];
+    eapply Forall_forall in HForall;
+    eauto.
+Qed.
+
+Definition Forall_map_inv A B P f xs := proj1 (Forall_map_iff A B P f xs).
+Definition Forall_map A B P f xs := proj2 (Forall_map_iff A B P f xs).
 
 Lemma StronglySorted_app A le (xs : list A) ys :
   StronglySorted le xs ->
@@ -46,8 +65,8 @@ Proof.
 Qed.
 
 Lemma StronglySorted_rev A le (xs : list A) :
-  StronglySorted le xs ->
-  StronglySorted (fun x y => le y x) (rev xs).
+  StronglySorted (fun x y => le y x) xs ->
+  StronglySorted le (rev xs).
 Proof.
   induction 1 as [| ? ? ? ? HForall ]; simpl.
   - constructor.
@@ -57,192 +76,242 @@ Proof.
     eauto.
 Qed.
 
-Module MergeSort (Import X : TotalTransitiveLeBool').
+Lemma StronglySorted_rev_inv A le (xs : list A) :
+  StronglySorted (fun x y => le y x) (rev xs) ->
+  StronglySorted le xs.
+Proof.
+  intros.
+  rewrite <- rev_involutive.
+  apply StronglySorted_rev.
+  assumption.
+Qed.
+
+Fact Permutation_fold_right A xss : forall ys ys',
+  Permutation ys ys' ->
+  Permutation (ys ++ fold_right (@app A) [] xss) (fold_right (@app A) ys' (rev (map (@rev A) xss))).
+Proof.
+  induction xss; simpl in *; intros ? ? HPermutation.
+  - rewrite app_nil_r.
+    eauto.
+  - rewrite app_assoc.
+    rewrite fold_right_app.
+    simpl.
+    apply IHxss.
+    eapply Permutation_trans.
+    + apply Permutation_app_comm.
+    + apply Permutation_app; eauto.
+      apply Permutation_rev.
+Qed.
+
+Module MergeSort.
   Local Coercion is_true : bool >-> Sortclass.
 
   Local Hint Constructors Permutation.
 
-  Definition merge : forall xs, StronglySorted leb xs ->
-    forall ys, StronglySorted leb ys ->
-    forall acc,
-    { ws | exists zs, ws = rev zs ++ acc /\ StronglySorted leb zs /\ Permutation zs (xs ++ ys) }.
-  Proof.
-    refine (fix merge xs :=
-      match xs as xs0 return
-        StronglySorted leb xs0 ->
-        forall ys, StronglySorted leb ys ->
-        forall acc,
-        { ws | exists zs, ws = rev zs ++ acc
-            /\ StronglySorted leb zs
-            /\ Permutation zs (xs0 ++ ys) } with
-      | [] => fun _ ys _ acc => exist _ (rev_append ys acc) _
-      | x :: xs' => fun _ =>
-          fix merge' ys :=
-            match ys with
-            | [] => fun _ acc => exist _ (rev_append xs' (x :: acc)) _
-            | y :: ys' => fun _ acc => 
-                if Sumbool.sumbool_of_bool (x <=? y) then
-                  let (zs, H) := merge xs' _ (y :: ys') _ (x :: acc) in
-                  exist _ zs _
-                else
-                  let (zs, _) := merge' ys' _ (y :: acc) in
-                  exist _ zs _
-            end
-      end); try clear merge';
-      try match goal with
-      | H : exists _, _ |- _ => destruct H
-      end;
-      [ exists ys | exists (x :: xs') | | | exists (x :: x0) | | exists (y :: x0) ];
-      repeat (simpl in *; match goal with
-      | H : StronglySorted _ (_ :: _) |- _ => inversion H; clear H; subst
-      | H : _ /\ _ |- _ => destruct H
-      | _ => rewrite app_nil_r in *
-      | _ => rewrite rev_append_rev in *
-      | _ => rewrite <- app_assoc
-      | _ => split
-      | _ => apply SSorted_cons
-      end; subst);
-      eauto;
-      repeat match goal with
-      | H : Forall ?P ?l |- _ =>
-          assert (forall x, In x l -> P x)
-            by (apply Forall_forall; eauto);
-          clear H
-      | |- Forall _ _ =>
-          apply Forall_forall; intros
-      end.
-    - apply (Permutation_in _ H0) in H3.
-      apply in_app_iff in H3.
-      destruct H3 as [| HIn]; eauto.
-      inversion HIn; subst; eauto.
-      eapply leb_trans; eauto.
-    - destruct (leb_total x y); [ congruence |].
-      apply (Permutation_in _ H0) in H3.
-      apply in_app_iff with (l := x :: xs') in H3.
-      destruct H3 as [HIn |]; eauto.
-      inversion HIn; subst; eauto.
-      eapply leb_trans; eauto.
-    - apply Permutation_cons_app with (l1 := x :: xs').
-      eauto.
-  Defined.
+  Section Tools.
+    Variable t : Set.
+    Variable leb : t -> t -> bool.
+    Hypothesis leb_total : forall x y, leb x y \/ leb y x.
+    Hypothesis leb_trans : Transitive leb.
+    Hint Resolve leb_trans.
 
-  Definition meld : forall xss,
-    Forall (StronglySorted leb) xss ->
-    forall acc,
-    { zss | exists xss', zss = rev xss' ++ acc /\ length xss' = div2 (S (length xss))
-        /\ Forall (StronglySorted leb) xss'
-        /\ Permutation (fold_right (@app _) [] xss') (fold_right (@app _) [] xss) }.
-  Proof.
-    refine (fix meld xss :=
-      match xss with
-      | [] => fun _ acc => exist _ acc _
-      | [xs] => fun _ acc => exist _ (xs :: acc) _
-      | xs :: xs' :: xss' => fun _ acc =>
-          let (ys, _) := merge xs _ xs' _ [] in
-          let (yss, _) := meld xss' _ (rev ys :: acc) in
-          exist _ yss _
-      end); clear meld;
-      repeat match goal with
-      | H : exists _, _ |- _ => destruct H
-      end;
-      [ exists (@nil (list t)) | exists [xs] | | | | exists (rev ys :: x) ];
-      repeat (simpl in *; match goal with
-      | _ => rewrite app_nil_r in *
-      | _ => rewrite rev_involutive in *
-      | H : Forall _ (_ :: _) |- _ =>
-          inversion H; clear H; subst
-      | H : _ /\ _ |- _ => destruct H
-      | _ => rewrite <- app_assoc
-      | _ => split
-      end; subst); eauto.
-    rewrite app_assoc.
-    apply Permutation_app; eauto.
-  Defined.
+    Definition merge :
+      forall xs, StronglySorted leb xs ->
+      forall ys, StronglySorted leb ys ->
+      forall acc,
+      { ws | exists zs, ws = rev zs ++ acc /\ StronglySorted leb zs /\ Permutation zs (xs ++ ys) }.
+    Proof.
+      refine (fix merge xs :=
+        match xs as xs0 return
+          StronglySorted leb xs0 ->
+          forall ys, StronglySorted leb ys ->
+          forall acc,
+          { ws | exists zs, ws = rev zs ++ acc
+              /\ StronglySorted leb zs
+              /\ Permutation zs (xs0 ++ ys) } with
+        | [] => fun _ ys _ acc => exist _ (rev_append ys acc) _
+        | x :: xs' => fun _ =>
+            fix merge' ys :=
+              match ys with
+              | [] => fun _ acc => exist _ (rev_append xs' (x :: acc)) _
+              | y :: ys' => fun _ acc => 
+                  if Sumbool.sumbool_of_bool (leb x y) then
+                    let (zs, H) := merge xs' _ (y :: ys') _ (x :: acc) in
+                    exist _ zs _
+                  else
+                    let (zs, _) := merge' ys' _ (y :: acc) in
+                    exist _ zs _
+              end
+        end); try clear merge';
+        try match goal with
+        | H : exists _, _ |- _ => destruct H
+        end;
+        [ exists ys | exists (x :: xs') | | | exists (x :: x0) | | exists (y :: x0) ];
+        repeat (simpl in *; match goal with
+        | H : StronglySorted _ (_ :: _) |- _ => inversion H; clear H; subst
+        | H : _ /\ _ |- _ => destruct H
+        | _ => rewrite app_nil_r in *
+        | _ => rewrite rev_append_rev in *
+        | _ => rewrite <- app_assoc
+        | _ => split
+        | _ => apply SSorted_cons
+        end; subst);
+        eauto;
+        repeat match goal with
+        | H : Forall ?P ?l |- _ =>
+            assert (forall x, In x l -> P x)
+              by (apply Forall_forall; eauto);
+            clear H
+        | |- Forall _ _ =>
+            apply Forall_forall; intros
+        end.
+      - apply (Permutation_in _ H0) in H3.
+        apply in_app_iff in H3.
+        destruct H3 as [| HIn]; eauto.
+        inversion HIn; subst; eauto.
+      - destruct (leb_total x y); [ congruence |].
+        apply (Permutation_in _ H0) in H3.
+        apply in_app_iff with (l := x :: xs') in H3.
+        destruct H3 as [HIn |]; eauto.
+        inversion HIn; subst; eauto.
+      - apply Permutation_cons_app with (l1 := x :: xs').
+        eauto.
+    Defined.
 
-  Definition merge_sort xs :
+    Definition meld : forall xss,
+      Forall (StronglySorted leb) xss ->
+      forall acc,
+      { zss | exists xss', zss = rev (map (@rev t) xss') ++ acc /\ length xss' = div2 (S (length xss))
+          /\ Forall (StronglySorted leb) xss'
+          /\ Permutation (fold_right (@app _) [] xss') (fold_right (@app _) [] xss) }.
+    Proof.
+      refine (fix meld xss :=
+        match xss with
+        | [] => fun _ acc => exist _ acc _
+        | [xs] => fun _ acc => exist _ (rev xs :: acc) _
+        | xs :: xs' :: xss' => fun _ acc =>
+            let (ys, _) := merge xs _ xs' _ [] in
+            let (yss, _) := meld xss' _ (ys :: acc) in
+            exist _ yss _
+        end); clear meld;
+        repeat match goal with
+        | H : exists _, _ |- _ => destruct H
+        end;
+        [ exists (@nil (list t)) | exists [xs] | | | | exists (x0 :: x) ];
+        repeat (simpl in *; match goal with
+        | _ => rewrite app_nil_r in *
+        | _ => rewrite rev_involutive in *
+        | H : Forall _ (_ :: _) |- _ =>
+            inversion H; clear H; subst
+        | H : _ /\ _ |- _ => destruct H
+        | _ => rewrite <- app_assoc
+        | _ => split
+        end; subst); eauto.
+      rewrite app_assoc.
+      apply Permutation_app; eauto.
+    Defined.
+  End Tools.
+
+  Definition merge_sort (t : Set) (leb : t -> t -> bool)
+    (leb_total : forall x y, leb x y \/ leb y x)
+    (leb_trans : Transitive leb) xs :
     { xs' | StronglySorted leb xs' /\ Permutation xs' xs }.
   Proof.
     refine (let (xs', _) := Fix
         (well_founded_ltof _ (@length _))
         (fun xss =>
-          Forall (StronglySorted leb) xss ->
+          forall is_rev : bool,
+          Forall (StronglySorted (if is_rev then fun x y => leb y x else leb)) xss ->
           Permutation (fold_right (@app _) [] xss) xs ->
           { xs' | StronglySorted leb xs' /\ Permutation xs' xs })
         (fun xss =>
           match xss with
-          | [] => fun _ _ _ => exist _ [] _
-          | [xs] => fun _ _ _ => exist _ xs _
-          | xs :: ys :: xss => fun iter_meld _ _ =>
-              let (xss', _) := meld (xs :: ys :: xss) _ [] in
-              iter_meld (rev xss') _ _ _
+          | [] => fun _ _ _ _ => exist _ [] _
+          | [xs] => fun _ is_rev _ _ =>
+              if Sumbool.sumbool_of_bool is_rev then exist _ (rev xs) _
+              else exist _ xs _
+          | xs :: ys :: xss => fun iter_meld is_rev _ _ =>
+              if Sumbool.sumbool_of_bool is_rev then
+                let (xss', _) :=
+                  meld _ (fun x y => leb y x) _ _ (xs :: ys :: xss) _ [] in
+                  iter_meld xss' _ (negb is_rev) _ _
+              else
+                let (xss', _) := meld _ leb _ _ (xs :: ys :: xss) _ [] in
+                iter_meld xss' _ (negb is_rev) _ _
           end)
-        (map (fun x => [x]) xs) _ _ in
+        (map (fun x => [x]) xs) false _ _ in
       exist _ xs' _);
       repeat (simpl in *; match goal with
       | _ => rewrite app_nil_r in *
-      | _ => rewrite rev_involutive in *
-      | H : Forall _ (_ :: _) |- _ =>
-          inversion H; clear H; subst
+      | _ => apply StronglySorted_rev
+      | _ => apply Forall_rev
+      | _ => apply Forall_map
+      | H : Forall _ (_ :: _) |- _ => inversion H; clear H; subst
+      | H : Forall _ (_ ++ _) |- _ => apply Forall_app_iff in H
       | H : _ /\ _ |- _ => destruct H
       | H : exists _, _ |- _ => destruct H
       | _ => split
+      | H : context [if ?b then _ else _] |- _ => destruct b
+      | H : Forall _ ?l |- Forall _ ?l => eapply Forall_impl; [| apply H ]
       end; subst);
       eauto.
+    - eapply Permutation_trans.
+      + apply Permutation_rev.
+      + rewrite rev_involutive.
+        eauto.
     - unfold ltof.
       simpl in *.
+      rewrite rev_length.
+      rewrite map_length.
       destruct (length xss0).
       + omega.
       + rewrite H.
         apply le_n_S.
         apply lt_div2 with (n := S (S n)).
         omega.
+    - apply Permutation_sym.
+      eapply Permutation_trans.
+      + apply Permutation_sym.
+        eauto.
+      + eapply Permutation_trans.
+        * apply Permutation_sym.
+          eauto.
+        * apply Permutation_fold_right with (A := t) (ys := []).
+          eauto.
+    - unfold ltof.
+      simpl in *.
+      rewrite rev_length.
+      rewrite map_length.
+      destruct (length xss0).
+      + omega.
+      + rewrite H.
+        apply le_n_S.
+        apply lt_div2 with (n := S (S n)).
+        omega.
+    - apply Permutation_sym.
+      eapply Permutation_trans.
+      + apply Permutation_sym.
+        eauto.
+      + eapply Permutation_trans.
+        * apply Permutation_sym.
+          eauto.
+        * apply Permutation_fold_right with (A := t) (ys := []).
+          eauto.
     - apply Forall_forall.
-      intros ? HIn.
-      apply in_map_iff in HIn.
-      destruct HIn as [? []].
-      subst.
       eauto.
     - induction xs; simpl; eauto.
   Defined.
 End MergeSort.
 
-Module Nat_as_TTLB <: TotalTransitiveLeBool.
-  Let t := nat.
-
-  Definition leb m n :=
-    if le_dec m n then true
-    else false.
-
-  Definition leb_total m n :
-    leb m n = true \/ leb n m = true.
-  Proof.
-    unfold leb.
-    destruct (le_dec m n);
-      destruct (le_dec n m);
-        solve [ eauto | omega ].
-  Qed.
-
-  Definition leb_trans l m n :
-    leb l m = true ->
-    leb m n = true ->
-    leb l n = true.
-  Proof.
-    unfold leb.
-    intros.
-    destruct (le_dec l m);
-      destruct (le_dec m n);
-        destruct (le_dec l n);
-          solve [ congruence | omega ].
-  Qed.
-End Nat_as_TTLB.
-
-Module NatSort := MergeSort Nat_as_TTLB.
 Extract Inductive bool => "bool" ["true" "false"].
+Extract Inductive sumbool => "bool" ["true" "false"].
 Extract Inductive list => "list" ["[]" "(::)"].
 Extract Constant map => "List.map".
 Extract Constant app => "( @ )".
 Extract Constant rev => "List.rev".
 Extract Constant rev_append => "List.rev_append".
+Extract Constant Sumbool.sumbool_of_bool => "(fun b => b)".
+Extract Constant negb => "not".
 Extraction (* "mergeSort.ml" *) MergeSort.
 
 (* FUCKIN' HEAVY COMPUTATION *)
